examples/pseudo_bool/array/colorProgScript.sml
@@ -1,0 +1,775 @@
+(*
+  Color encode and checker
+*)
+Theory colorProg
+Ancestors
+  basis_ffi pbc_normalise graphProg color graph_basic
+    npbc_parseProg pb_parse
+Libs
+  preamble basis
+
+val _ = translation_extends"graphProg";
+
+val res = translate enc_string_def;
+val res = translate color_obj_def;
+val res = translate FOLDN_def;
+val res = translate annot_string_def;
+
+val _ = use_sub_check true;
+
+val res = translate gen_constraint_def;
+
+val _ = use_sub_check false;
+
+val res = translate full_encode_eq;
+
+(* Translation for parsing an OPB file *)
+val r = translate pb_parseTheory.nocomment_line_def;
+val r = translate parse_op_def;
+val r = translate parse_constraint_def;
+val r = translate parse_annot_def;
+val r = translate parse_annot_constraint_def;
+val r = translate parse_constraints_def;
+
+val r = translate parse_obj_def;
+val r = translate parse_obj_maybe_def;
+val r = translate parse_var_raw_def;
+val r = translate parse_vars_raw_def;
+val r = translate parse_pres_def;
+val r = translate parse_pres_maybe_def;
+val r = translate parse_obj_pres_maybe_def;
+val r = translate parse_pbf_toks_def;
+
+Quote add_cakeml:
+  fun parse_pbf_full f =
+  (case TextIO.inputAllTokensFile #"\n" f blanks tokenize of
+    None => Inl (notfound_string f)
+  | Some lines =>
+  (case parse_pbf_toks lines of
+    None => Inl (noparse_string f "OPB")
+  | Some res => Inr res
+  ))
+End
+
+val inputAllTokensFile_spec_specialize =
+  inputAllTokensFile_spec
+  |> Q.GEN `f` |> Q.SPEC`blanks`
+  |> Q.GEN `fv` |> Q.SPEC`blanks_v`
+  |> Q.GEN `g` |> Q.ISPEC`tokenize`
+  |> Q.GEN `gv` |> Q.ISPEC`tokenize_v`
+  |> Q.GEN `a` |> Q.ISPEC`SUM_TYPE STRING_TYPE INT`
+  |> REWRITE_RULE [blanks_v_thm,tokenize_v_thm] ;
+
+Definition get_annot_fml_def:
+  get_annot_fml fs f =
+  if inFS_fname fs f then
+    parse_pbf (all_lines_file fs f)
+  else NONE
+End
+
+Theorem parse_pbf_full_spec:
+  STRING_TYPE f fv ∧
+  validArg f ∧
+  hasFreeFD fs
+  ⇒
+  app (p:'ffi ffi_proj) ^(fetch_v"parse_pbf_full"(get_ml_prog_state()))
+    [fv]
+    (STDIO fs)
+    (POSTv v.
+    & (∃err. (SUM_TYPE STRING_TYPE annot_prob_TYPE)
+    (case get_annot_fml fs f of
+      NONE => INL err
+    | SOME res => INR res) v) * STDIO fs)
+Proof
+  rw[]>>
+  xcf"parse_pbf_full"(get_ml_prog_state())>>
+  reverse (Cases_on `STD_streams fs`) >- (fs [TextIOProofTheory.STDIO_def] \\ xpull) >>
+  reverse (Cases_on`consistentFS fs`) >- (
+    fs [STDIO_def,IOFS_def,wfFS_def,consistentFS_def]
+    \\ xpull \\ metis_tac[]) >>
+  xlet`(POSTv sv. &OPTION_TYPE (LIST_TYPE (LIST_TYPE (SUM_TYPE STRING_TYPE INT)))
+            (if inFS_fname fs f then
+               SOME(MAP (MAP tokenize o tokens blanks) (all_lines_file fs f))
+             else NONE) sv * STDIO fs)`
+  >- (
+    xapp_spec inputAllTokensFile_spec_specialize >>
+    xsimpl>>
+    simp[pb_parseTheory.blanks_def]>>
+    fs[FILENAME_def,validArg_def,blanks_v_thm]>>
+    first_x_assum (irule_at Any)>>
+    first_x_assum (irule_at Any)>>
+    first_x_assum (irule_at Any)>>
+    qexists_tac`emp`>>xsimpl)>>
+  simp[get_annot_fml_def]>>
+  IF_CASES_TAC>>fs[OPTION_TYPE_def]>>xmatch
+  >- (
+    xlet_autop>>
+    `toks = (MAP tokenize ∘ tokens blanks)` by
+      rw[FUN_EQ_THM,toks_def]>>
+    rw[parse_pbf_def]>>
+    qmatch_goalsub_abbrev_tac`option_CASE AAA`>>
+    Cases_on`AAA`>>
+    fs[OPTION_TYPE_def]
+    >- (
+      xmatch >>
+      xlet_autop>>
+      xcon>>xsimpl>>
+      simp[SUM_TYPE_def]>>metis_tac[])>>
+    xmatch>>
+    xcon>>
+    xsimpl>>
+    simp[SUM_TYPE_def])>>
+  xlet_autop>>
+  xcon>>xsimpl>>
+  simp[SUM_TYPE_def]>>metis_tac[]
+QED
+
+(* parse input from f and run encoder into pbc *)
+Quote add_cakeml:
+  fun parse_and_enc f =
+  case parse_dimacs f of
+    Inl err => Inl err
+  | Inr g =>
+    Inr (full_encode (fst g) g)
+End
+
+Theorem parse_and_enc_spec:
+  STRING_TYPE f fv ∧
+  validArg f ∧
+  hasFreeFD fs
+  ⇒
+  app (p:'ffi ffi_proj) ^(fetch_v"parse_and_enc"(get_ml_prog_state()))
+    [fv]
+    (STDIO fs)
+    (POSTv v.
+    STDIO fs *
+    & ∃res.
+       SUM_TYPE STRING_TYPE
+         (PAIR_TYPE
+            (OPTION_TYPE (PAIR_TYPE
+              (LIST_TYPE (PAIR_TYPE INT (PBC_LIT_TYPE STRING_TYPE)))
+            INT))
+            (LIST_TYPE
+              (PAIR_TYPE
+              (OPTION_TYPE STRING_TYPE)
+              (PAIR_TYPE PBC_PBOP_TYPE (PAIR_TYPE (LIST_TYPE (PAIR_TYPE INT (PBC_LIT_TYPE STRING_TYPE))) INT))))
+            ) res v ∧
+       case res of
+        INL err =>
+          get_graph_dimacs fs f = NONE
+      | INR objf =>
+        ∃g.
+          get_graph_dimacs fs f = SOME g ∧
+          full_encode (FST g) g = objf)
+Proof
+  rw[]>>
+  xcf"parse_and_enc"(get_ml_prog_state())>>
+  xlet_autop>>
+  every_case_tac>>fs[SUM_TYPE_def]>>xmatch
+  >- (
+    xcon>>xsimpl>>
+    qexists_tac`INL err`>>simp[SUM_TYPE_def])>>
+  rpt xlet_autop>>
+  xcon>>xsimpl >>
+  rename1`_ (full_encode _ g)`>>
+  qexists_tac`INR (full_encode (FST g) g)`>>
+  simp[SUM_TYPE_def,PAIR_TYPE_def]
+QED
+
+Definition mk_prob_def:
+  mk_prob objf = (NONE,objf):mlstring list option #
+    ((int # mlstring pbc$lit) list # int) option #
+    (mlstring option # (pbop # (int # mlstring pbc$lit) list # int)) list
+End
+
+val res = translate mk_prob_def;
+
+Definition check_unsat_1_sem_def:
+  check_unsat_1_sem fs f1 out ⇔
+  case get_graph_dimacs fs f1 of
+    NONE => out = strlit ""
+  | SOME g =>
+    out = concat (print_annot_prob (mk_prob (full_encode (FST g) g)))
+End
+
+Quote add_cakeml:
+  fun check_unsat_1 f1 =
+  case parse_and_enc f1 of
+    Inl err => TextIO.output TextIO.stdErr err
+  | Inr objf =>
+    TextIO.print_list (print_annot_prob (mk_prob objf))
+End
+
+Theorem check_unsat_1_spec:
+  STRING_TYPE f1 f1v ∧ validArg f1 ∧
+  hasFreeFD fs
+  ⇒
+  app (p:'ffi ffi_proj) ^(fetch_v"check_unsat_1"(get_ml_prog_state()))
+    [f1v]
+    (STDIO fs)
+    (POSTv uv. &UNIT_TYPE () uv *
+    SEP_EXISTS out err.
+      STDIO (add_stdout (add_stderr fs err) out) *
+      &(check_unsat_1_sem fs f1 out))
+Proof
+  rw[check_unsat_1_sem_def]>>
+  xcf "check_unsat_1" (get_ml_prog_state ())>>
+  reverse (Cases_on `STD_streams fs`) >- (fs [TextIOProofTheory.STDIO_def] \\ xpull) >>
+  xlet_autop>>
+  Cases_on`res`>>fs[SUM_TYPE_def]
+  >- (
+    xmatch>>
+    xapp_spec output_stderr_spec \\ xsimpl>>
+    asm_exists_tac>>xsimpl>>
+    qexists_tac`emp`>>qexists_tac`fs`>>xsimpl>>
+    fs[STD_streams_add_stderr, STD_streams_stdout,add_stdo_nil]>>
+    rw[]>>
+    qexists_tac`x`>>xsimpl)>>
+  xmatch>>
+  xlet_autop>>
+  xlet_autop>>
+  xapp_spec print_list_spec>>xsimpl>>
+  asm_exists_tac>>xsimpl>>
+  qexists_tac`emp`>>qexists_tac`fs`>>xsimpl>>
+  rw[]>>
+  qexists_tac`strlit ""`>>
+  simp[STD_streams_stderr,add_stdo_nil]>>
+  xsimpl
+QED
+
+val _ = translate parse_col_header_def;
+val _ = translate strip_num_def;
+val _ = translate parse_col_line_def;
+val _ = translate parse_col_lines_def;
+val _ = translate mk_col_def;
+val _ = translate parse_col_toks_def;
+
+Quote add_cakeml:
+  fun parse_col f =
+  (case TextIO.inputAllTokensFile #"\n" f blanks tokenize_num of
+    None => Inl (notfound_string f)
+  | Some lines =>
+  (case parse_col_toks lines of
+    None => Inl (noparse_string f "COLOR")
+  | Some x =>
+      Inr x
+    ))
+End
+
+(* get_col *)
+Definition get_col_def:
+  get_col fs f =
+  if inFS_fname fs f then
+    parse_col (all_lines_file fs f)
+  else NONE
+End
+
+val inputAllTokensFile_spec_specialize_num =
+  inputAllTokensFile_spec
+  |> Q.GEN `f` |> Q.SPEC`blanks`
+  |> Q.GEN `fv` |> Q.SPEC`blanks_v`
+  |> Q.GEN `g` |> Q.ISPEC`tokenize_num`
+  |> Q.GEN `gv` |> Q.ISPEC`tokenize_num_v`
+  |> Q.GEN `a` |> Q.ISPEC`SUM_TYPE STRING_TYPE NUM`
+  |> REWRITE_RULE [blanks_v_thm,tokenize_num_v_thm] ;
+
+Theorem parse_col_spec:
+  STRING_TYPE f fv ∧
+  validArg f ∧
+  hasFreeFD fs
+  ⇒
+  app (p:'ffi ffi_proj) ^(fetch_v"parse_col"(get_ml_prog_state()))
+    [fv]
+    (STDIO fs)
+    (POSTv v.
+    & (∃err. SUM_TYPE STRING_TYPE (PAIR_TYPE NUM (NUM --> NUM))
+      (case get_col fs f of
+        NONE => INL err
+      | SOME res => INR res) v) * STDIO fs)
+Proof
+  rw[]>>
+  xcf"parse_col"(get_ml_prog_state())>>
+  reverse (Cases_on `STD_streams fs`) >- (fs [TextIOProofTheory.STDIO_def] \\ xpull) >>
+  reverse (Cases_on`consistentFS fs`) >- (
+    fs [STDIO_def,IOFS_def,wfFS_def,consistentFS_def]
+    \\ xpull \\ metis_tac[]) >>
+  xlet`(POSTv sv. &OPTION_TYPE (LIST_TYPE (LIST_TYPE (SUM_TYPE STRING_TYPE NUM)))
+            (if inFS_fname fs f then
+               SOME(MAP (MAP tokenize_num o tokens blanks) (all_lines_file fs f))
+             else NONE) sv * STDIO fs)`
+  >- (
+    xapp_spec inputAllTokensFile_spec_specialize_num >>
+    xsimpl>>
+    simp[pb_parseTheory.blanks_def]>>
+    fs[FILENAME_def,validArg_def,blanks_v_thm]>>
+    first_x_assum (irule_at Any)>>
+    first_x_assum (irule_at Any)>>
+    first_x_assum (irule_at Any)>>
+    qexists_tac`emp`>>xsimpl)>>
+  simp[get_col_def]>>
+  reverse IF_CASES_TAC>>fs[OPTION_TYPE_def]>>xmatch
+  >- (
+    xlet_autop>>
+    xcon>>xsimpl>>
+    simp[SUM_TYPE_def]>>metis_tac[])>>
+  xlet_autop>>
+  `toks_num = (MAP tokenize_num ∘ tokens blanks)` by
+    metis_tac[toks_num_def,ETA_AX,o_DEF]>>
+  Cases_on`parse_col (all_lines_file fs f)`>>
+  gvs[parse_col_def,OPTION_TYPE_def]
+  >- (
+    xmatch >>
+    xlet_autop>>
+    xcon>>xsimpl>>
+    simp[SUM_TYPE_def]>>metis_tac[])>>
+  xmatch>>
+  xcon>>xsimpl>>
+  simp[SUM_TYPE_def]
+QED
+
+(* Pretty print conclusion *)
+Definition color_eq_str_def:
+  color_eq_str (n:num) =
+  strlit "s VERIFIED CHROMATIC NUMBER = " ^
+    toString n ^ strlit"\n"
+End
+
+Definition color_bound_str_def:
+  color_bound_str (l:num) (u:num) =
+  strlit "s VERIFIED CHROMATIC NUMBER BOUND "^
+    toString l ^ strlit " <= NUM COL <= " ^
+    toString u ^ strlit"\n"
+End
+
+Definition print_color_str_def:
+  print_color_str lbg ubg =
+  if lbg = ubg
+  then color_eq_str ubg
+  else color_bound_str lbg ubg
+End
+
+Definition color_sem_def:
+  color_sem g lb k f ⇔
+  is_k_color k f g ∧
+  if lb = k then
+    min_color_size g = k
+  else
+    (∀k f.
+        is_k_color k f g ⇒ lb ≤ k)
+End
+
+Definition check_unsat_4_sem_def:
+  check_unsat_4_sem fs fg fc out ⇔
+  (out ≠ strlit"" ⇒
+  ∃g lb k f.
+    get_graph_dimacs fs fg = SOME g ∧
+    good_graph g ∧
+    get_col fs fc = SOME (k,f) ∧
+    out = print_color_str lb k ∧
+    color_sem g lb k f)
+End
+
+val _ = translate check_k_color_aux_def;
+val _ = translate check_k_color_def;
+
+val _ = translate MAX_LIST_def;
+val _ = translate parse_cu_def;
+val _ = translate guess_n_def;
+val _ = translate mk_key_def;
+
+Theorem mk_key_side[local]:
+  mk_key_side x
+Proof
+  rw[fetch "-" "mk_key_side_def"]>>
+  CCONTR_TAC>>fs[]
+QED
+
+val _ = mk_key_side |> update_precondition;
+
+val _ = translate lazy_constraint_aux_def;
+val _ = translate lazy_constraint_def;
+
+val _ = translate lazy_encode_def;
+val _ = translate lazy_color_obj_def;
+val res = translate lazy_full_encode_def;
+
+(* f1: graph, f2: opb, f3: proof, f4: coloring *)
+Quote add_cakeml:
+  fun parse_and_check f1 f2 f4 =
+  case parse_dimacs f1 of
+    Inl err => Inl err
+  | Inr g =>
+  case parse_col f4 of
+    Inl err => Inl err
+  | Inr (k,f) =>
+  if check_k_color k f g
+  then
+    case parse_pbf_full f2 of
+      Inl err => Inl err
+    | Inr prob =>
+      case lazy_full_encode g prob of
+        None =>
+        Inl "Input OPB not subset of encoding"
+      | Some n => Inr (k, (n, prob))
+  else
+    Inl "Invalid coloring"
+End
+
+Definition parse_and_check_sem_def:
+  parse_and_check_sem fs f1 f2 f4 res ⇔
+  (∀k n prob.
+    res = INR (k,n,prob) ⇒
+    ∃g f.
+      get_graph_dimacs fs f1 = SOME g ∧
+      good_graph g ∧
+      get_col fs f4 = SOME (k,f) ∧
+      is_k_color k f g ∧
+      lazy_full_encode g prob = SOME n)
+End
+
+Theorem parse_and_check_spec:
+  STRING_TYPE f1 f1v ∧ validArg f1 ∧
+  STRING_TYPE f2 f2v ∧ validArg f2 ∧
+  STRING_TYPE f4 f4v ∧ validArg f4 ∧
+  hasFreeFD fs
+  ⇒
+  app (p:'ffi ffi_proj) ^(fetch_v"parse_and_check"(get_ml_prog_state()))
+    [f1v; f2v; f4v]
+    (STDIO fs)
+    (POSTv v.
+      STDIO fs *
+      &(∃res.
+        SUM_TYPE STRING_TYPE (PAIR_TYPE NUM (PAIR_TYPE NUM annot_prob_TYPE)) res v ∧
+        parse_and_check_sem fs f1 f2 f4 res))
+Proof
+  rw[parse_and_check_sem_def]>>
+  xcf"parse_and_check"(get_ml_prog_state())>>
+  reverse (Cases_on `STD_streams fs`) >- (fs [TextIOProofTheory.STDIO_def] \\ xpull) >>
+  xlet_autop>>
+  Cases_on`get_graph_dimacs fs f1`>>
+  fs[SUM_TYPE_def]>>
+  xmatch
+  >- (
+    xcon>>xsimpl>>
+    qexists_tac`INL err`>>
+    simp[SUM_TYPE_def])>>
+  xlet_autop>>
+  Cases_on`get_col fs f4`>>
+  fs[SUM_TYPE_def]
+  >- (
+    xmatch>>
+    xcon>>xsimpl>>
+    qexists_tac`INL err`>>
+    simp[SUM_TYPE_def]
+  )>>
+  rename1`xx = (_,_)`>>
+  Cases_on`xx`>>
+  fs[PAIR_TYPE_def]>>
+  xmatch>>
+  xlet_autop>>
+  reverse xif
+  >- (
+    xcon>>xsimpl>>
+    qexists_tac`INL «Invalid coloring»`>>
+    simp[SUM_TYPE_def])>>
+  xlet_autop>>
+  Cases_on`get_annot_fml fs f2`>>
+  fs[SUM_TYPE_def]>>
+  xmatch
+  >- (
+    xcon>>xsimpl>>
+    qexists_tac`INL err`>>
+    simp[SUM_TYPE_def])>>
+  xlet_autop>>
+  gvs[npbc_arrayProgTheory.OPTION_TYPE_SPLIT]>>
+  xmatch
+  >- (
+    xcon>>xsimpl>>
+    qexists_tac`INL «Input OPB not subset of encoding»`>>
+    simp[SUM_TYPE_def])>>
+  xlet_autop>>
+  xlet_autop>>
+  xcon>>
+  xsimpl>>
+  gvs[get_graph_dimacs_def,AllCaseEqs(),mk_prob_def,pb_parseTheory.strip_annot_prob_def]>>
+  drule parse_dimacs_good_graph>>
+  rw[]>>
+  rename1`check_k_color k f g`>>
+  rename1`lazy_full_encode _ prob = SOME n`>>
+  qexists_tac`INR (k,n,prob)`>>
+  simp[SUM_TYPE_def,PAIR_TYPE_def]>>
+  metis_tac[check_k_color_is_k_color]
+QED
+
+Definition map_concl_to_string_def:
+  (map_concl_to_string k n (INL s) = (INL s)) ∧
+  (map_concl_to_string k n (INR (out,bnd,c)) =
+    case conv_concl n c of
+      SOME lb => INR (print_color_str lb k)
+    | NONE => INL (strlit "c Unexpected conclusion type for min coloring problem.\n"))
+End
+
+val res = translate conv_concl_def;
+val res = translate color_eq_str_def;
+val res = translate color_bound_str_def;
+val res = translate print_color_str_def;
+val res = translate map_concl_to_string_def;
+
+Quote add_cakeml:
+  fun check_unsat_4 f1 f2 f3 f4 =
+  case parse_and_check f1 f2 f4 of
+    Inl err => TextIO.output TextIO.stdErr err
+  | Inr (k,(n,prob)) =>
+    let
+      val prob = strip_annot_prob prob
+      val probt = default_prob in
+      (case
+        map_concl_to_string k n
+          (check_unsat_top_norm False prob probt f3) of
+        Inl err => TextIO.output TextIO.stdErr err
+      | Inr s => TextIO.print s)
+    end
+End
+
+Theorem check_unsat_4_spec:
+  STRING_TYPE f1 f1v ∧ validArg f1 ∧
+  STRING_TYPE f2 f2v ∧ validArg f2 ∧
+  STRING_TYPE f3 f3v ∧ validArg f3 ∧
+  STRING_TYPE f4 f4v ∧ validArg f4 ∧
+  hasFreeFD fs
+  ⇒
+  app (p:'ffi ffi_proj) ^(fetch_v"check_unsat_4"(get_ml_prog_state()))
+    [f1v; f2v; f3v; f4v]
+    (STDIO fs)
+    (POSTv uv. &UNIT_TYPE () uv *
+    SEP_EXISTS out err.
+      STDIO (add_stdout (add_stderr fs err) out) *
+      &(check_unsat_4_sem fs f1 f4 out))
+Proof
+  rw[check_unsat_4_sem_def]>>
+  xcf "check_unsat_4" (get_ml_prog_state ())>>
+  reverse (Cases_on `STD_streams fs`) >- (fs [TextIOProofTheory.STDIO_def] \\ xpull) >>
+  xlet_autop>>
+  Cases_on`res`>>fs[SUM_TYPE_def]
+  >- (
+    xmatch>>
+    xapp_spec output_stderr_spec \\ xsimpl>>
+    asm_exists_tac>>xsimpl>>
+    qexists_tac`emp`>>xsimpl>>
+    qexists_tac`fs`>>xsimpl>>
+    rw[]>>
+    qexists_tac`strlit""`>>xsimpl>>rw[]>>
+    qexists_tac`x`>>xsimpl>>rw[]>>
+    fs[STD_streams_add_stderr, STD_streams_stdout,add_stdo_nil]>>
+    xsimpl)>>
+  `?k n prob. y = (k,n,prob)` by metis_tac[PAIR]>>
+  fs[PAIR_TYPE_def]>>
+  xmatch>>
+  xlet_autop>>
+  assume_tac npbc_parseProgTheory.default_prob_v_thm>>
+  xlet`POSTv v.
+    STDIO fs *
+    &prob_TYPE default_prob v`
+  >-
+    (xvar>>xsimpl)>>
+  xlet`POSTv v. STDIO fs * &BOOL F v`
+  >-
+    (xcon>>xsimpl)>>
+  drule npbc_parseProgTheory.check_unsat_top_norm_spec>>
+  qpat_x_assum`prob_TYPE (strip_annot_prob _) _`assume_tac>>
+  disch_then drule>>
+  qpat_x_assum`prob_TYPE default_prob _`assume_tac>>
+  disch_then drule>>
+  strip_tac>>
+  xlet_auto
+  >- (
+    xsimpl>>
+    fs[validArg_def]>>
+    metis_tac[])>>
+  xlet_autop>>
+  gvs[AllCasePreds(),SUM_TYPE_def]
+  >- (
+    fs[map_concl_to_string_def,SUM_TYPE_def]>>
+    xmatch>>
+    xapp_spec output_stderr_spec \\ xsimpl>>
+    asm_exists_tac>>xsimpl>>
+    qexists_tac`emp`>>xsimpl>>
+    qexists_tac`fs`>>xsimpl>>
+    rw[]>>
+    qexists_tac`strlit ""`>>
+    rename1`add_stderr _ err`>>
+    qexists_tac`err`>>xsimpl>>rw[]>>
+    fs[STD_streams_add_stderr, STD_streams_stdout,add_stdo_nil]>>
+    xsimpl)>>
+  fs[map_concl_to_string_def]>>
+  every_case_tac>>fs[SUM_TYPE_def]>>xmatch
+  >- (
+    xapp_spec output_stderr_spec \\ xsimpl>>
+    asm_exists_tac>>xsimpl>>
+    qexists_tac`emp`>>xsimpl>>
+    qexists_tac`fs`>>xsimpl>>
+    rw[]>>
+    qexists_tac`strlit ""`>>
+    rename1`add_stderr _ err`>>
+    qexists_tac`err`>>xsimpl>>rw[]>>
+    fs[STD_streams_add_stderr, STD_streams_stdout,add_stdo_nil]>>
+    xsimpl)
+  >- (
+    xapp>>xsimpl>>
+    asm_exists_tac>>simp[]>>
+    qexists_tac`emp`>>qexists_tac`fs`>>xsimpl>>
+    rw[]>>
+    qexists_tac`print_color_str x k`>>simp[]>>
+    qexists_tac`strlit ""`>>
+    rw[]>>simp[STD_streams_stderr,add_stdo_nil]>>
+    xsimpl>>
+    gvs[parse_and_check_sem_def,color_sem_def]>>
+    rename1`print_color_str lb k`>>
+    qexists_tac`lb`>>simp[]>>
+    (drule_at Any) lazy_full_encode_sem_concl>>
+    disch_then drule>>
+    PairCases_on`prob`>>
+    disch_then drule>>
+    fs[strip_annot_prob_def]>>
+    rw[]>>fs[]>>
+    metis_tac[min_color_size_eq])
+QED
+
+Definition usage_string_def:
+  usage_string = strlit "Usage: cake_pb_color <DIMACS graph file> <OPB file> <PB proof file> <coloring file>\n"
+End
+
+val r = translate usage_string_def;
+
+Quote add_cakeml:
+  fun main u =
+  let
+    val cl = CommandLine.arguments ()
+    val l = List.length cl
+  in
+    if l = 1 then check_unsat_1 (el 0 cl)
+    else if l = 4 then check_unsat_4 (el 0 cl) (el 1 cl) (el 2 cl) (el 3 cl)
+    else TextIO.output TextIO.stdErr (mk_usage_string usage_string)
+  end
+End
+
+Definition main_sem_def:
+  main_sem fs cl out =
+  if LENGTH cl = 2 then
+    check_unsat_1_sem fs (EL 1 cl) out
+  else if LENGTH cl = 5 then
+    check_unsat_4_sem fs (EL 1 cl) (EL 4 cl) out
+  else out = strlit ""
+End
+
+Theorem STDIO_refl:
+  STDIO A ==>>
+  STDIO A * GC
+Proof
+  xsimpl
+QED
+
+Theorem LENGTH_EQ_4:
+  LENGTH ls = 4 ⇔
+  ∃a b c d. ls = [a;b;c;d]
+Proof
+  Cases_on`ls`>>rw[]>>
+  Cases_on`t`>>rw[]>>
+  Cases_on`t'`>>rw[]>>
+  Cases_on`t`>>rw[]>>
+  rw[ADD1]
+QED
+
+Theorem main_spec:
+  hasFreeFD fs
+  ⇒
+  app (p:'ffi ffi_proj) ^(fetch_v"main"(get_ml_prog_state()))
+    [Conv NONE []]
+    (COMMANDLINE cl * STDIO fs)
+    (POSTv uv. &UNIT_TYPE () uv *
+    COMMANDLINE cl *
+    SEP_EXISTS out err.
+      STDIO (add_stdout (add_stderr fs err) out) *
+      &(main_sem fs cl out))
+Proof
+  rw[main_sem_def]>>
+  xcf"main"(get_ml_prog_state())>>
+  reverse (Cases_on `STD_streams fs`) >- (fs [TextIOProofTheory.STDIO_def] \\ xpull) >>
+  reverse(Cases_on`wfcl cl`) >- (fs[COMMANDLINE_def] \\ xpull)>>
+  rpt xlet_autop >>
+  Cases_on `cl` >- fs[wfcl_def] >>
+  fs[]>>xif
+  >- (
+    xlet_auto
+    >- (
+      xsimpl>>
+      simp[npbc_arrayProgTheory.el_side_def]>>
+      CCONTR_TAC>>gvs[])>>
+    xapp>>xsimpl>>
+    rpt(first_x_assum (irule_at Any)>>xsimpl)>>
+    gvs[LENGTH_EQ_1,wfcl_def]>>
+    rw[]>>metis_tac[STDIO_refl])>>
+  xlet_autop>>
+  xif
+  >- (
+    rpt (xlet_auto
+    >- (
+      xsimpl>>
+      simp[npbc_arrayProgTheory.el_side_def]>>
+      rw[]>>gvs[ADD1]>>
+      CCONTR_TAC>>gvs[quantHeuristicsTheory.CONS_EQ_REWRITE]))>>
+    xapp>>xsimpl>>
+    rpt(first_x_assum (irule_at Any)>>xsimpl)>>
+    gvs[LENGTH_EQ_4,wfcl_def]>>
+    rw[]>>metis_tac[STDIO_refl])>>
+  simp[ADD1]>>
+  assume_tac (theorem "usage_string_v_thm")>>
+  xlet_autop>>
+  xapp_spec output_stderr_spec \\ xsimpl>>
+  rename1`COMMANDLINE cl`>>
+  qexists_tac`COMMANDLINE cl`>>xsimpl>>
+  qexists_tac `mk_usage_string usage_string` >>
+  simp [] >>
+  qexists_tac`fs`>>xsimpl>>
+  rw[]>>
+  fs[STD_streams_add_stderr, STD_streams_stdout,add_stdo_nil]>>
+  metis_tac[STDIO_refl]
+QED
+
+Theorem main_whole_prog_spec2:
+   hasFreeFD fs ⇒
+   whole_prog_spec2 main_v cl fs NONE
+     (λfs'. ∃out err.
+        fs' = add_stdout (add_stderr fs err) out ∧
+        main_sem fs cl out)
+Proof
+  rw[basis_ffiTheory.whole_prog_spec2_def]
+  \\ match_mp_tac (MP_CANON (DISCH_ALL (MATCH_MP app_wgframe (UNDISCH main_spec))))
+  \\ xsimpl
+  \\ rw[PULL_EXISTS]
+  \\ qexists_tac`add_stdout (add_stderr fs x') x`
+  \\ xsimpl
+  \\ qexists_tac`x`
+  \\ qexists_tac`x'`
+  \\ xsimpl
+  \\ simp[GSYM add_stdo_with_numchars,with_same_numchars]
+QED
+
+local
+
+val name = "main"
+val (sem_thm,prog_tm) =
+  whole_prog_thm (get_ml_prog_state()) name (UNDISCH main_whole_prog_spec2)
+Definition main_prog_def:
+  main_prog = ^prog_tm
+End
+
+in
+
+Theorem main_semantics =
+  sem_thm
+  |> REWRITE_RULE[GSYM main_prog_def]
+  |> DISCH_ALL
+  |> SIMP_RULE(srw_ss())[GSYM CONJ_ASSOC,AND_IMP_INTRO];
+
+end
