examples/pseudo_bool/array/compilation/colorCompileScript.sml
@@ -1,0 +1,15 @@
+(*
+  Compiles the min color + PB checker
+*)
+Theory colorCompile
+Ancestors
+  colorProg
+Libs
+  preamble eval_cake_compile_x64Lib eval_cake_compile_arm8Lib
+
+Theorem color_compiled =
+  eval_cake_compile_x64 "" main_prog_def "cake_pb_color.S";
+
+Theorem color_compiled_arm8 =
+  eval_cake_compile_arm8 "arm8_" main_prog_def "cake_pb_color_arm8.S";
+
