examples/pseudo_bool/array/compilation/proofs/colorProofScript.sml
@@ -1,0 +1,119 @@
+(*
+  Compose the semantics theorem and the compiler correctness
+  theorem with the compiler evaluation theorem to produce end-to-end
+  correctness theorem that reaches final machine code.
+*)
+Theory colorProof
+Ancestors
+  semanticsProps backendProof x64_configProof TextIOProof
+  colorProg color colorCompile
+Libs
+  preamble
+
+val cake_pb_color_io_events_def = new_specification("cake_pb_color_io_events_def",["cake_pb_color_io_events"],
+  main_semantics |> Q.GENL[`cl`,`fs`]
+  |> SIMP_RULE bool_ss [SKOLEM_THM,Once(GSYM RIGHT_EXISTS_IMP_THM)]);
+
+val (cake_pb_color_sem,cake_pb_color_output) = cake_pb_color_io_events_def |> SPEC_ALL |> UNDISCH |> SIMP_RULE std_ss [GSYM PULL_EXISTS]|> CONJ_PAIR
+val (cake_pb_color_not_fail,cake_pb_color_sem_sing) = cake_pb_color_sem
+  |> SRULE [color_compiled,ml_progTheory.prog_syntax_ok_semantics]
+  |> MATCH_MP semantics_prog_Terminate_not_Fail |> CONJ_PAIR
+
+val compile_correct_applied =
+  MATCH_MP compile_correct (cj 1 color_compiled)
+  |> SIMP_RULE(srw_ss())[LET_THM,ml_progTheory.init_state_env_thm,GSYM AND_IMP_INTRO]
+  |> C MATCH_MP cake_pb_color_not_fail
+  |> C MATCH_MP x64_backend_config_ok
+  |> REWRITE_RULE[cake_pb_color_sem_sing,AND_IMP_INTRO]
+  |> REWRITE_RULE[Once (GSYM AND_IMP_INTRO)]
+  |> C MATCH_MP (CONJ(UNDISCH x64_machine_config_ok)(UNDISCH x64_init_ok))
+  |> DISCH(#1(dest_imp(concl x64_init_ok)))
+  |> REWRITE_RULE[AND_IMP_INTRO]
+
+Theorem cake_pb_color_compiled_thm =
+  CONJ compile_correct_applied cake_pb_color_output
+  |> DISCH_ALL
+  (* |> check_thm *)
+
+(* Prettifying the standard parts of all the theorems *)
+Definition installed_x64_def:
+  installed_x64 ((code, data, cfg) :
+      (word8 list # word64 list # 64 backend$config))
+    mc ms
+  <=>
+    ?cbspace data_sp.
+      is_x64_machine_config mc /\
+      installed
+        code cbspace
+        data data_sp
+        cfg.lab_conf.ffi_names
+        (heap_regs x64_backend_config.stack_conf.reg_names) mc
+        cfg.lab_conf.shmem_extra ms
+End
+
+Definition cake_pb_color_code_def:
+  cake_pb_color_code = (code, data, info)
+End
+
+(* A standard run of cake_pb_color
+  satisfying all the default assumptions *)
+Definition cake_pb_color_run_def:
+  cake_pb_color_run cl fs mc ms ⇔
+  wfcl cl ∧ wfFS fs ∧ STD_streams fs ∧ hasFreeFD fs ∧
+  installed_x64 cake_pb_color_code mc ms
+End
+
+Theorem machine_code_sound:
+  cake_pb_color_run cl fs mc ms ⇒
+  machine_sem mc (basis_ffi cl fs) ms ⊆
+    extend_with_resource_limit
+      {Terminate Success (cake_pb_color_io_events cl fs)} ∧
+  ∃out err.
+    extract_fs fs (cake_pb_color_io_events cl fs) =
+      SOME (add_stdout (add_stderr fs err) out) ∧
+    (out ≠ strlit"" ⇒
+      ∃g.
+        get_graph_dimacs fs (EL 1 cl) = SOME g ∧
+        (
+          (LENGTH cl = 2 ∧
+            out = concat (print_annot_prob (mk_prob (full_encode (FST g) g)))) ∨
+          (LENGTH cl = 5 ∧
+            ∃k f.
+              get_col fs (EL 4 cl) = SOME (k,f) ∧
+              is_k_color k f g ∧
+              (out = color_eq_str (min_color_size g) ∨
+              ∃l.
+                out = color_bound_str l k ∧
+                (∀k' f'. is_k_color k' f' g ⇒ l ≤ k')))
+        )
+    )
+Proof
+  strip_tac>>
+  fs[installed_x64_def,cake_pb_color_code_def,cake_pb_color_run_def]>>
+  drule cake_pb_color_compiled_thm>>
+  simp[AND_IMP_INTRO]>>
+  disch_then drule>>
+  disch_then (qspecl_then [`ms`,`mc`,`data_sp`,`cbspace`] mp_tac)>>
+  simp[]>> strip_tac>>
+  fs[main_sem_def]>>
+  pop_assum mp_tac>>
+  rpt (IF_CASES_TAC)>>
+  strip_tac
+  >- (
+    qexists_tac`out`>>qexists_tac`err`>>simp[]>>
+    fs[check_unsat_1_sem_def]>>
+    every_case_tac>>gvs[])
+  >- (
+    qexists_tac`out`>>qexists_tac`err`>>simp[]>>
+    fs[check_unsat_4_sem_def]>>
+    strip_tac>>
+    gvs[]>>
+    qpat_x_assum`color_sem _ _ _ _` mp_tac>>
+    simp[color_sem_def,print_color_str_def]>>
+    rw[]>>
+    metis_tac[])>>
+  metis_tac[]
+QED
+
+val chk = machine_code_sound |> check_thm;
+
