examples/pseudo_bool/array/compilation/proofs/README.md
@@ -10,6 +10,11 @@ Compose the semantics theorem and the compiler correctness
 theorem with the compiler evaluation theorem to produce end-to-end
 correctness theorem that reaches final machine code.
 
+[colorProofScript.sml](colorProofScript.sml):
+Compose the semantics theorem and the compiler correctness
+theorem with the compiler evaluation theorem to produce end-to-end
+correctness theorem that reaches final machine code.
+
 [mccisProofScript.sml](mccisProofScript.sml):
 Compose the semantics theorem and the compiler correctness
 theorem with the compiler evaluation theorem to produce end-to-end
